@prefix : <http://purl.org/net/wf-motifs#> .
@prefix owl: <http://www.w3.org/2002/07/owl#> .
@prefix rdf: <http://www.w3.org/1999/02/22-rdf-syntax-ns#> .
@prefix xml: <http://www.w3.org/XML/1998/namespace> .
@prefix xsd: <http://www.w3.org/2001/XMLSchema#> .
@prefix rdfs: <http://www.w3.org/2000/01/rdf-schema#> .
@base <http://purl.org/net/wf-motifs> .

<http://purl.org/net/wf-motifs> rdf:type owl:Ontology ;
                                 rdfs:comment "Workflow Motif Ontology, created by Daniel Garijo, Pinar Alper and Khalid Belhajjame"@en ,
                                              "This ontology is based on the paper: Common Motifs in Scientific Workflows:An Empirical Analysis, by Daniel Garijo, Pinar Alper, Khalid Belhajjame, Oscar Corcho, Yolanda Gil and Carole Goble" ;
                                 rdfs:label "Workflow Motif Ontology"@en ;
                                 owl:versionInfo "Version 1.01" .

#################################################################
#    Object Properties
#################################################################

###  http://purl.org/net/wf-motifs#implementsMotif
:implementsMotif rdf:type owl:ObjectProperty ;
                 rdfs:range :Motif ;
                 rdfs:comment "This object property is used to annotate a step in the workflow, a group of steps, a subworkflow, or a workflow with a motif." ;
                 rdfs:label "implements motif"@en .


###  http://purl.org/net/wf-motifs#implementsOperationMotif
:implementsOperationMotif rdf:type owl:ObjectProperty ;
                          rdfs:subPropertyOf :implementsMotif ;
                          rdfs:range :OperationMotif ;
                          rdfs:comment "Object property that connects a, workflow step with its correspondent OperationMotif."@en ;
                          rdfs:label "implements operation motif"@en .


###  http://purl.org/net/wf-motifs#implementsWorkflowMotif
:implementsWorkflowMotif rdf:type owl:ObjectProperty ;
                         rdfs:subPropertyOf :implementsMotif ;
                         rdfs:range :WorkflowMotif ;
                         rdfs:comment "Object property that relates a Workflow to its correspondent motif"@en ;
                         rdfs:label "implements workflow motif"@en .


#################################################################
#    Classes
#################################################################

###  http://purl.org/net/wf-motifs#AsynchronousInvocation
:AsynchronousInvocation rdf:type owl:Class ;
                        rdfs:subClassOf :IntraWorkflowMotif ;
                        rdfs:comment "Certain activities such as analysis or visualizations could be performed through interaction with stateful (web) services that allow for creation of jobs over remote grid environments. These are typically performed via invocation of multiple operations at a service endpoint. "@en ;
                        rdfs:label "Asynchronous invocation"@en .


###  http://purl.org/net/wf-motifs#AtomicWorkflow
:AtomicWorkflow rdf:type owl:Class ;
                rdfs:subClassOf :InterWorkflowMotif ;
                rdfs:comment "Motif used to characetrize the workflows that perform an atomic unit of functionality, which effectively requires no sub-workflow usage. Typically these workflows are designed to be included in other work- flows. Atomic workflows are the main mechanism of modularizing functionality wthin scientific workflows." ;
                rdfs:label "Atomic workflow"@en .


###  http://purl.org/net/wf-motifs#CompositeWorkflow
:CompositeWorkflow rdf:type owl:Class ;
                   rdfs:subClassOf :InterWorkflowMotif ;
                   rdfs:comment "This motif refers to all those workflows that have one or more sub-workflows included in them (in some cases, these sub-workflows offer different views of the global workflow). "@en ;
                   rdfs:label "Composite workflow"@en .


###  http://purl.org/net/wf-motifs#ComputationalStep
:ComputationalStep rdf:type owl:Class ;
                   rdfs:subClassOf :IntraWorkflowMotif ;
                   rdfs:comment "This motif is used to refer to activities that do not require human inputs during their execution." ;
                   rdfs:label "Computational step"@en .


###  http://purl.org/net/wf-motifs#DataAnalysis
:DataAnalysis rdf:type owl:Class ;
              rdfs:subClassOf <http://purl.org/net/wf-motifsl#DataCreation> ;
              rdfs:comment "Motif that refers to a broad category of tasks in diverse domains. An important number of workflows are designed with the purpose of analyzing different features of input data, ranging from simple comparisons between the datasets to complex protein analysis to see whether two molecules can be docked successfully or not. "@en ;
              rdfs:label "Data analysis"@en .


###  http://purl.org/net/wf-motifs#DataCleaning
:DataCleaning rdf:type owl:Class ;
              rdfs:subClassOf :OperationMotif ;
              rdfs:comment "Steps for cleaning and curating data. Typically these steps are undertaken by sophisticated tooling/services, or by human interactions. A cleaning step essentially preserves and enriches the content of data (e.g., by a user’s annotation of a result with additional information, detecting and removing inconsistencies on the data, etc.)." ;
              rdfs:label "Data cleaning"@en .


###  http://purl.org/net/wf-motifs#DataMovement
:DataMovement rdf:type owl:Class ;
              rdfs:subClassOf :OperationMotif ;
              rdfs:comment "Certain analysis activities that are performed via external tools or services require the submission of data to a location accessible by the service/tool (i.e., a web or a local directory respectively). In such cases the workflow contains dedicated step(s) for the upload/transfer of data to these locations. The same applies to the outputs, in which case a data download/retrieval step is used to chain the data to the next steps of the workflow."@en ;
              rdfs:label "Data movement"@en .


###  http://purl.org/net/wf-motifs#DataPreparation
:DataPreparation rdf:type owl:Class ;
                 rdfs:subClassOf :OperationMotif ;
                 rdfs:comment "Data, as it is originally retrieved, may need several transformations before being able to be used in a workflow step. The steps in the workflow performing such transformations can be annotated used the Data Preparation motif."@en ;
                 rdfs:label "Data Preparation"@en .


###  http://purl.org/net/wf-motifs#DataRetrieval
:DataRetrieval rdf:type owl:Class ;
               rdfs:subClassOf <http://purl.org/net/wf-motifsl#DataCreation> ;
               rdfs:comment "Workflows exploit heterogeneous data sources, remote databases, repositories or other web resources mostly exposed via SOAP or REST services. Scientific data deposited in these repositories are retrieved through query and retrieval steps inside workflows. Certain tasks within the workflow are responsible for retrieving data from such exter- nal source into the workflow environment." ;
               rdfs:label "Data retrieval"@en .


###  http://purl.org/net/wf-motifs#DataVisualization
:DataVisualization rdf:type owl:Class ;
                   rdfs:subClassOf <http://purl.org/net/wf-motifsl#DataCreation> ;
                   rdfs:comment "Being able to show the results is as important as producing them in some workflows. Scientists use visualizations to show the conclusions of their experiments and to take important decisions in the pipeline itself. Therefore certain steps in workflows are dedicated to generation of plots and graph outputs from input data."@en ;
                   rdfs:label "Data Visualization"@en .


###  http://purl.org/net/wf-motifs#FormatTransformation
:FormatTransformation rdf:type owl:Class ;
                      rdfs:subClassOf :UnstructuredDataPreparation ;
                      rdfs:comment "Workflows that bring together multiple access or analysis activities usually contain steps for format transformations. Typically, these steps, also known as ”Shims”, preserve the contents of data, while converting its representation format."@en ;
                      rdfs:label "Format transformation"@en .


###  http://purl.org/net/wf-motifs#Group
:Group rdf:type owl:Class ;
       rdfs:subClassOf :StructuredDataPreparation ;
       rdfs:comment "Motif that refers to the step or set of steps that reorganize the input into different groups. For example, grouping a table by a certain category."@en ;
       rdfs:label "Group"@en .


###  http://purl.org/net/wf-motifs#HumanInteraction
:HumanInteraction rdf:type owl:Class ;
                  rdfs:subClassOf :IntraWorkflowMotif ;
                  rdfs:comment "Motif is used to characetrize the activities that require human inputs during their execution."@en ;
                  rdfs:label "Human interaction"@en .


###  http://purl.org/net/wf-motifs#InputAugmentation
:InputAugmentation rdf:type owl:Class ;
                   rdfs:subClassOf :UnstructuredDataPreparation ;
                   rdfs:comment "Motif that refers to the step or set of steps dedicated to generate aggregation of multiple parameters and scripts for tools and external services."@en ;
                   rdfs:label "Input augmentation"@en .


###  http://purl.org/net/wf-motifs#InterWorkflowMotif
:InterWorkflowMotif rdf:type owl:Class ;
                    rdfs:subClassOf :WorkflowMotif ;
                    rdfs:comment "Motif observed among different workflows."@en ;
                    rdfs:label "Inter-workflow motif"@en .


###  http://purl.org/net/wf-motifs#InternalMacro
:InternalMacro rdf:type owl:Class ;
               rdfs:subClassOf :IntraWorkflowMotif ;
               rdfs:comment "Motif that refers to those groups of steps in the workflow that correspond to repetitive patterns of combining tasks. "@en ;
               rdfs:label "Internal macro"@en .


###  http://purl.org/net/wf-motifs#IntraWorkflowMotif
:IntraWorkflowMotif rdf:type owl:Class ;
                    rdfs:subClassOf :WorkflowMotif ;
                    rdfs:comment "Category of motifs observed within a workflow."@en ;
                    rdfs:label "Intra-workflow motif"@en .


###  http://purl.org/net/wf-motifs#Join
:Join rdf:type owl:Class ;
      rdfs:subClassOf :StructuredDataPreparation ;
      rdfs:comment "Motif that refers to a step or a set of steps that aggregate their contents into a single output. Both intputs generally have the same type"@en ;
      rdfs:label "Join"@en .


###  http://purl.org/net/wf-motifs#Merge
:Merge rdf:type owl:Class ;
       rdfs:subClassOf :UnstructuredDataPreparation ;
       rdfs:comment "Motif that refers to the step of steps in the workflow aggregating information from heterogeneous and unstructured sources"@en ;
       rdfs:label "Merge"@en .


###  http://purl.org/net/wf-motifs#Motif
:Motif rdf:type owl:Class ;
       rdfs:comment "A motif is a domain independent conceptual abstraction of one or more steps of the workflow"@en ;
       rdfs:label "Motif"@en .


###  http://purl.org/net/wf-motifs#OperationMotif
:OperationMotif rdf:type owl:Class ;
                rdfs:subClassOf :Motif ;
                rdfs:comment "An operation motif describes the data manipulation and/or transformation carried out by a step in the workflow, a collection of steps in the workflow or a subworkflow"@en ;
                rdfs:label "Operation motif"@en .


###  http://purl.org/net/wf-motifs#OutputExtraction
:OutputExtraction rdf:type owl:Class ;
                  rdfs:subClassOf :UnstructuredDataPreparation ;
                  rdfs:comment "Motif that refers to the step or set of steps in the workflow that retrieve only the relevant portion from the the output of a previous step. For example, retrieving the tag value of an XML fragment."@en ;
                  rdfs:label "Output extraction"@en .


###  http://purl.org/net/wf-motifs#Sort
:Sort rdf:type owl:Class ;
      rdfs:subClassOf :StructuredDataPreparation ;
      rdfs:comment "Motif that refers to the step or set of steps ordering the input by certain parameter. For example, a quicksort algorithm that takes an unorderd vector and produces a sorted output."@en ;
      rdfs:label "Sort"@en .


###  http://purl.org/net/wf-motifs#StructuredDataPreparation
:StructuredDataPreparation rdf:type owl:Class ;
                           rdfs:subClassOf :DataPreparation ;
                           rdfs:comment "Data preparation motifs that require the some of all of the inputs to be structured in tables, excel files, etc."@en ;
                           rdfs:label "Structured data preparation"@en .


###  http://purl.org/net/wf-motifs#SynchronousInvocaton
:SynchronousInvocaton rdf:type owl:Class ;
                      rdfs:subClassOf :IntraWorkflowMotif ;
                      rdfs:comment "Motif that requires a single step for performing a service call or tool invocation."@en ;
                      rdfs:label "Synchronous invocation"@en .


###  http://purl.org/net/wf-motifs#UnstructuredDataPreparation
:UnstructuredDataPreparation rdf:type owl:Class ;
                             rdfs:subClassOf :DataPreparation ;
                             rdfs:comment "Data preparation motifs that don't require some of all of the inputs to be structured in tables, excel files, etc."@en ;
                             rdfs:label "Unstructured data preparation"@en .


###  http://purl.org/net/wf-motifs#WorkflowMotif
:WorkflowMotif rdf:type owl:Class ;
               rdfs:subClassOf :Motif ;
               rdfs:comment "A workflow motif describes how an operation motif is realized (i.e., implemented) within a workflow."@en ,
                            "Workflow motif"@en .


###  http://purl.org/net/wf-motifs#WorkflowOverload
:WorkflowOverload rdf:type owl:Class ;
                  rdfs:subClassOf :InterWorkflowMotif ;
                  rdfs:comment "Motif used to characetrize workflows that are used to operate over different input parameter types. An example is performing an analysis over a String input parameter, or performing it over the contents of a specified File. Overloading is a direct response to the heterogeneity of environments in which workflows are used."@en ;
                  rdfs:label "Workflow overload"@en .


###  http://purl.org/net/wf-motifsl#DataCreation
<http://purl.org/net/wf-motifsl#DataCreation> rdf:type owl:Class ;
                                              rdfs:subClassOf :OperationMotif ;
                                              rdfs:comment "Motif that represents a step or set of steps where new data is created by the workflow. It serves to highlight the main functionality of the workflow."@en ;
                                              rdfs:label "Data creation"@en .


###  http://purl.org/net/wf-motifsl#Filter
<http://purl.org/net/wf-motifsl#Filter> rdf:type owl:Class ;
                                        rdfs:subClassOf :StructuredDataPreparation ;
                                        rdfs:comment "Motif that refers to a filtering step or set of steps. For example, A file filtered by a set of set of keywords, a table filtered by a threshold, etc."@en ;
                                        rdfs:label """Filter
"""@en .


###  http://purl.org/net/wf-motifsl#Split
<http://purl.org/net/wf-motifsl#Split> rdf:type owl:Class ;
                                       rdfs:subClassOf :UnstructuredDataPreparation ;
                                       rdfs:comment "Motif that refers to the step or steps in the workflow that separate an input into different outputs."@en ;
                                       rdfs:label "Split"@en .


###  Generated by the OWL API (version 5.1.14) https://github.com/owlcs/owlapi/
